lean/FlowAnalysis/VariableModel/JoinTestedImpl.lean
@@ -1,0 +1,14 @@
+module
+public import Batteries.Data.List.Basic
+public import Batteries.Data.List.Lemmas
+public import FlowAnalysis.Types
+
+namespace FlowAnalysis.VariableModel
+
+variable {τ : Type} [DartTypeRepr τ]
+
+-- TODO: placeholder
+@[expose]
+public def joinTestedImpl (ts₁ ts₂ : List τ) : List τ := ts₁ ∪ ts₂
+
+end FlowAnalysis.VariableModel
